%----------------------------------------------------------------------------------------
%	PACKAGES AND OTHER DOCUMENT CONFIGURATIONS
%----------------------------------------------------------------------------------------
\documentclass[10pt]{article}
\usepackage{amsmath}
\usepackage{amssymb}
\usepackage{enumitem}
\usepackage{amsfonts}
\usepackage{graphicx}
\usepackage{caption}
\usepackage{threeparttable}
\usepackage{lipsum}
\usepackage{multirow}
\newcommand\tab[1][1cm]{\hspace*{#1}}

%----------------------------------------------------------------------------------------
%	TITLE
%----------------------------------------------------------------------------------------
\title{DS 598 DEEP LEARNING}
\author{Sungjoon Park (BUID: U38522578)}
\date{Jan. 30st, 2024}

\begin{document}
\maketitle

\setlength{\parindent}{0cm}
\setlength{\parskip}{2mm}

%----------------------------------------------------------------------------------------
%	BODY
%----------------------------------------------------------------------------------------
\textbf{Problem Set 2}

\begin{enumerate}

% Problem 1
\item

	$L(\phi)=\sum_{i=1}^{I}(\phi_0+\phi_1x_i-y_i)^2$
	
	with respect to $\phi_0$
	\begin{align*}
	\frac{\partial L(\phi)}{\partial \phi_0} &= 2\sum_{i=1}^{I}(\phi_0+\phi_1x_i-y_i) \\
	&= 2I\phi_0+2\phi_1\sum_{i=1}^Ix_i-2\sum_{i=1}^Iy_i
	\end{align*}
	
	with respect to $\phi_1$
	\begin{align*}
	\frac{\partial L(\phi)}{\partial \phi_1} &= 2\sum_{i=1}^{I}x_i(\phi_0+\phi_1x_i-y_i) \\
	&= 2\phi_0\sum_{i=1}^Ix_i+2\phi_1\sum_{i=1}^Ix_i^2-2\sum_{i=1}^Ix_iy_i
	\end{align*}



% Problem 2	
\item

	First Order Condition \\
	with respect to $\phi_0$
	\begin{align*}
	\frac{\partial L(\phi)}{\partial \phi_0} &= 2I\phi_0+2\phi_1\sum_{i=1}^Ix_i-2\sum_{i=1}^Iy_i \\
	&= 0
	\end{align*}
	
	$$I\phi_0+\phi_1\sum_{i=1}^Ix_i-\sum_{i=1}^Iy_i=0$$
	
	\begin{align*}
	\phi_0^* &= \frac{1}{I}\sum_{i=1}^Iy_i-\frac{\phi_1}{I}\sum_{i=1}^Ix_i \\
	&= \bar{y}-\phi_1\bar{x}
	\end{align*}
	
	with respect to $\phi_1$
	\begin{align*}
	\frac{\partial L(\phi)}{\partial \phi_1} &= 2\sum_{i=1}^{I}x_i(\phi_0+\phi_1x_i-y_i) \\
	\intertext{Since $\phi_0^*=\bar{y}-\phi_1\bar{x}$,}
	&= 2\sum_{i=1}^{I}x_i(\bar{y}-\phi_1\bar{x}+\phi_1x_i-y_i) \\
	&= 2\sum_{i=1}^{I}x_i(\phi_1(x_i-\bar{x})-(y_i-\bar{y})) \\
	&= 0
	\end{align*}
	
	\begin{align*}
	\phi_1^* &= \frac{\sum_{i=1}^{I}x_i(y_i-\bar{y})}{\sum_{i=1}^{I}x_i(x_i-\bar{x})}
	\end{align*}
	
	\begin{align*}
	\phi_0^* &= \bar{y}- \frac{\sum_{i=1}^{I}x_i(y_i-\bar{y})}{\sum_{i=1}^{I}x_i(x_i-\bar{x})}\bar{x}
	\end{align*}
	
	Second Order Condition \\
	with respect to $\phi_0$
	\begin{align*}
	\frac{\partial^2 L(\phi)}{\partial \phi_0^2} &= 2 > 0
	\end{align*}
	$\therefore$ $\phi_0*$ attains the global minimum.
	
	with respect to $\phi_1$
	$\because$ $\forall x_i$, $x_i \in \mathbb{R}^1$
	\begin{align*}
	\frac{\partial^2 L(\phi)}{\partial \phi_1^2} &= 2\sum_{i=1}^Ix_i^2 \geq 0
	\end{align*}
	
	$\therefore$ $\phi_1^*$ attains the global minimum.

\end{enumerate}

\end{document}